
\documentclass[12pt]{amsart}
\usepackage{geometry} % see geometry.pdf on how to lay out the page. There's lots.
\geometry{a4paper} % or letter or a5paper or ... etc
% \geometry{landscape} % rotated page geometry

% See the ``Article customise'' template for come common customisations

\title{Variance of MC versus TD}
\author{Ashwin Rao}
\date{} % delete this line to display the current date

%%% BEGIN DOCUMENT

\begin{document}
\maketitle
Assume a state is visited only once in an episode, so each of MC and TD update the value function for a state only once in an episode. Assume that for a given episode $k$, the variance of the value function for all states is the same. We will denote this variance as $y_k$ for MC and $z_k$ for TD. Assume $\gamma = 1$. Assume the variance of observed reward in any episode is a stationary value $x$. Assume we have $n$ time steps per episode (so, the variance of observed return in any episode is $nx$).

The MC update is:
$$V(S_t) \leftarrow V(S_t) + \alpha (G_t - V(S_t)) = (1-\alpha) V(S_t) + \alpha G_t$$

So, the Variance $y_k$ for MC in episode $k$ is given by:

$$y_k = (1-\alpha)^2 y_{k-1} + \alpha^2 nx = (1-\alpha)^2 ((1-\alpha)^2 y_{k-2} + \alpha^2 nx) + \alpha^2 nx = \ldots $$
$$ \ldots = (1-\alpha)^{2i} y_{k-i} + \alpha^2 nx\sum_{j=0}^{i-1} (1-\alpha)^{2j}$$

When $i=k, y_{k-i} = y_0 = 0$, and so,

$$y_k = \alpha^2 nx\sum_{j=0}^{k-1} (1-\alpha)^{2j}$$

For large enough $k$,

$$y_k = \frac {\alpha^2 nx} {1 - (1-\alpha)^2} = \frac {\alpha nx} {2 - \alpha}$$

The TD update is:
$$V(S_t) \leftarrow V(S_t) + \alpha (R_t + V(S_{t+1}) - V(S_t)) = (1-\alpha)V(S_t) + \alpha (R_t + V(S_{t+1}))$$

So, the Variance $z_k$ for TD in episode $k$ is given by:

$$z_k = (1-\alpha)^2 z_{k-1} + \alpha^2 (x + z_{k-1}) = ((1-\alpha)^2 + \alpha^2) z_{k-1}+ \alpha^2 x $$
$$ = ((1-\alpha)^2 +\alpha^2) (((1-\alpha)^2 +\alpha^2) z_{k-2} + \alpha^2 x) + \alpha^2 x = \ldots$$
$$ \ldots = ((1-\alpha)^2 + \alpha^2)^i z_{k-i} + \alpha^2 x \sum_{j=0}^{i-1} ((1-\alpha)^2 + \alpha^2)^j$$

When $i=k, z_{k-i} = z_0 = 0$, and so,

$$z_k = \alpha^2 x \sum_{j=0}^{k-1} ((1-\alpha)^2 + \alpha^2)^j$$

For large enough $k$,

$$z_k = \frac {\alpha^2 x} {1 - ((1-\alpha)^2 + \alpha^2)} = \frac {\alpha x} {2(1-\alpha)}$$

Comparing $y_k = \frac {\alpha nx} {2 - \alpha}$ with $z_k = \frac {\alpha x} {2(1-\alpha)}$, we see that for relatively small $\alpha$ and large $n$, 
$$y_k \approx n z_k$$
\end{document}